I2SFI/TestIntermediate.v
@@ -1,0 +1,233 @@
+Require Import Coq.Strings.Ascii.
+Require Import Coq.Strings.String.
+Require Import Coq.ZArith.ZArith.
+
+Require Import Common.Maps.
+Require Import Common.Definitions.
+Require Import Common.Values.
+Require Import Common.Memory.
+
+Require Import CompCert.Events.
+
+Require Export Lib.Monads.
+Require Import FunctionalExtensionality.
+
+Require Import Intermediate.Machine.
+Require Import Intermediate.GlobalEnv.
+Require Import Intermediate.CS.
+
+Import MonadNotations.
+Open Scope monad_scope.
+
+Inductive ExecutionError :=
+| MissingComponentId : Component.id -> ExecutionError
+| NegativePointerOffset : Pointer.t -> ExecutionError
+| LoadOutsideComponent : ExecutionError
+| LoadNotAddressInReg : ExecutionError
+| StoreOutsideComponent : ExecutionError
+| StoreNotAddressInReg : ExecutionError
+| JumpOutsideComponent : ExecutionError
+| JumpNotAddressInReg : ExecutionError
+| MissingJalLabel: ExecutionError
+| MissingLabel : ExecutionError
+| MissingBlock : Pointer.t -> ExecutionError
+| OffsetTooBig : Pointer.t -> ExecutionError
+| MemoryError : Pointer.t -> ExecutionError
+| NotIntInReg : ExecutionError
+| AllocNegativeBlockSize : ExecutionError
+| InvalidEnv : ExecutionError
+| NoInfo: ExecutionError
+.
+
+Inductive execution_state {A:Type} :=
+| Running : A -> execution_state
+| OutOfFuel : A -> execution_state
+| Halted : execution_state
+| Wrong : string -> ExecutionError -> execution_state.
+
+Instance exec_monad : Monad (@execution_state)
+  := {      
+      ret := fun {A:Type} (x:A) => @Running A x;
+      
+      bind := fun {A B:Type} (x : @execution_state A) (f : A -> @execution_state B) => 
+                match x with
+                | Running y => f y
+                | Wrong m err => Wrong m err
+                | Halted => Halted
+                | OutOfFuel y => f y
+                end
+    }.
+(* Not a real monad. Does not have right identity. *)
+
+Definition t : Type :=  (trace*CS.state).
+
+Definition lift {A} (x: option A) (msg : string) (err : ExecutionError) :=
+  match x with
+  | None  => (@Wrong A msg err)
+  | Some v => (@Running A v)
+  end.
+    
+Definition fail {A} (msg : string) (err : ExecutionError) :=
+  (@Wrong A msg err).
+
+
+Definition eval_step (G: global_env) (s: CS.state)  : (@execution_state t) :=
+  let '(gps, mem, regs, pc) := s in
+  (* fetch the next instruction to execute *)
+  do C_procs <- lift (PMap.find (Pointer.component pc) (genv_procedures G))
+        "Missing component"%string (MissingComponentId (Pointer.component pc));
+    match (PMap.find (Pointer.block pc) C_procs) with
+    | None => fail "Missing block"%string (MissingBlock pc)
+    | Some P_code => 
+      if Pointer.offset pc <? 0 then
+        fail "Negative offset"%string (NegativePointerOffset pc)
+      else
+        match nth_error P_code (Z.to_nat (Pointer.offset pc)) with
+        | None => fail "Offset too big"%string (OffsetTooBig pc)
+        | Some instr =>
+          (* decode and execute the instruction *)
+          match instr with
+          | ILabel l =>
+            ret (E0, (gps, mem, regs, Pointer.inc pc))
+          | INop =>
+            ret (E0, (gps, mem, regs, Pointer.inc pc))
+          | IConst v r =>
+            let regs' := Intermediate.Register.set r (imm_to_val v) regs in
+            ret (E0, (gps, mem, regs', Pointer.inc pc))
+          | IMov r1 r2 =>
+            let regs' := Intermediate.Register.set r2 (Intermediate.Register.get r1 regs) regs in
+            ret (E0, (gps, mem, regs', Pointer.inc pc))
+          | IBinOp op r1 r2 r3 =>
+            let regs' := Intermediate.Register.set
+                           r3 (eval_binop op (Intermediate.Register.get r1 regs)
+                                          (Intermediate.Register.get r2 regs))
+                           regs in
+            ret (E0, (gps, mem, regs', Pointer.inc pc))
+          | ILoad r1 r2 =>
+            match Intermediate.Register.get r1 regs with
+            | Ptr ptr =>
+              if Pos.eqb (Pointer.component ptr) (Pointer.component pc) then
+                do v <- lift (Memory.load mem ptr) "Memory load error" (MemoryError ptr);
+                  let regs' := Intermediate.Register.set r2 v regs in
+                  ret (E0, (gps, mem, regs', Pointer.inc pc))
+              else
+                fail "Load outside component"%string LoadOutsideComponent 
+            | _ => fail "Not a pointer value in address register"%string LoadNotAddressInReg
+            end
+          | IStore r1 r2 =>
+            match Intermediate.Register.get r1 regs with
+            | Ptr ptr =>
+              if Pos.eqb (Pointer.component ptr) (Pointer.component pc) then
+                do mem' <- lift (Memory.store mem ptr (Intermediate.Register.get r2 regs))
+                "Memory store error"%string (MemoryError ptr);
+                  ret (E0, (gps, mem', regs, Pointer.inc pc))
+              else
+                fail "Store outside component"%string StoreOutsideComponent
+            | _ => fail "Not a pointer value in address register"%string StoreNotAddressInReg
+            end
+          | IJal l =>
+            do pc' <- lift (find_label_in_component G pc l)
+              "Missing Jal label"%string MissingJalLabel;
+              let regs' :=  Intermediate.Register.set R_RA (Ptr (Pointer.inc pc)) regs in
+              @Running t (E0, (gps, mem, regs', pc'))
+          | IJump r =>
+            match Intermediate.Register.get r regs with
+            | Ptr pc' =>
+              if Pos.eqb (Pointer.component pc') (Pointer.component pc) then
+                ret (E0, (gps, mem, regs, pc'))
+              else
+                fail "Jump outside component"%string JumpOutsideComponent
+            | _ => fail "Not a pointer value in address register"%string JumpNotAddressInReg
+            end
+          | IBnz r l =>
+            match Intermediate.Register.get r regs with
+            | Int 0 =>
+              ret (E0, (gps, mem, regs, Pointer.inc pc))
+            | Int val =>
+              do pc' <- lift (find_label_in_procedure G pc l)
+                  "Missing Bnz label"%string MissingLabel;
+                ret (E0, (gps, mem, regs, pc'))
+            | _ => fail  "Bnz::Not int"%string NotIntInReg
+            end
+          | IAlloc rptr rsize =>
+            match Intermediate.Register.get rsize regs with
+            | Int size =>
+              if size <=? 0 then
+                fail  "Negative block size"%string AllocNegativeBlockSize
+              else
+                do (mem', ptr) <- lift (Memory.alloc mem (Pointer.component pc) (Z.to_nat size))
+                   "Alloc failed"%string (MemoryError pc);
+                let regs' := Intermediate.Register.set rptr (Ptr ptr) regs in
+                ret (E0, (gps, mem', regs', Pointer.inc pc))
+            | _ => fail  "Alloc::Not int"%string NotIntInReg
+            end
+          | ICall C' P =>
+            if negb (Pos.eqb (Pointer.component pc) C') then
+              if imported_procedure_b (genv_interface G) (Pointer.component pc) C' P then
+                do b <- lift (Intermediate.EntryPoint.get C' P (genv_entrypoints G))
+                    "Call::Incorrect environment"%string InvalidEnv;
+                  match Intermediate.Register.get R_COM regs with
+                  | Int rcomval =>
+                    let pc' := (C', b, 0) in
+                    let tr := [ECall (Pointer.component pc) P rcomval C'] in
+                    let res : t := (tr, (Pointer.inc pc :: gps,
+                                         mem,
+                                         Intermediate.Register.invalidate regs,
+                                         pc')) in
+                    ret res
+                  | _ => fail "Call::Missing register R_COM"%string NoInfo
+                  end
+              else
+                fail  "Call::procedure not imported"%string InvalidEnv
+            else
+              fail  "Call::same component"%string InvalidEnv
+          | IReturn =>
+            match gps with
+            | pc' :: gps' =>
+              if negb (Pos.eqb (Pointer.component pc) (Pointer.component pc')) then
+                match Intermediate.Register.get R_COM regs with
+                | Int rcomval =>
+                  let tr := [ERet (Pointer.component pc) rcomval (Pointer.component pc')] in
+                  ret (tr, (gps', mem, Intermediate.Register.invalidate regs, pc'))
+                | _ => fail  "Return::Missing register R_COM"%string InvalidEnv
+                end
+              else
+                fail  "Return::same component"%string InvalidEnv
+            | _ => fail "Empty Stack"%string InvalidEnv
+            end
+          | IHalt =>  Halted
+          end
+        end
+    end
+.
+
+Definition init_genv_and_state (p: Intermediate.program)
+           (input: value) : option (global_env * CS.state) :=
+  let '(mem, E, ps) := Intermediate.init_all p in
+  let G := {| genv_interface := Intermediate.prog_interface p;
+              genv_procedures := ps;
+              genv_entrypoints := E |} in
+  do b <- Intermediate.EntryPoint.get (fst (Intermediate.prog_main p))
+     (snd (Intermediate.prog_main p)) (genv_entrypoints G);
+  let regs := Intermediate.Register.set R_COM input Intermediate.Register.init in
+  ret (G, ([], mem, regs, (fst (Intermediate.prog_main p), b, 0))).
+
+Fixpoint execN (n: nat) (G: global_env) (tr:trace) (st: CS.state) : execution_state :=
+  match n with
+  | O => OutOfFuel (tr,st)
+  | S n' =>
+    match eval_step G st with
+    | Halted => Halted
+    | OutOfFuel s => OutOfFuel s
+    | Wrong msg err => Wrong msg err
+    | Running (ntr,nst) => execN n' G (tr++ntr) nst
+    end
+  end.
+
+Definition runp (p: Intermediate.program) (input: value) (fuel: nat) : execution_state :=
+  match init_genv_and_state p input with
+  | None => Wrong "Init failed" NoInfo
+  | Some (G, st) =>  execN fuel G E0 st
+  end.
+
+Close Scope monad_scope.
