TargetSFI/MachineGen.v
@@ -28,6 +28,7 @@ Require Import Common.Maps.
 
 Require Import TargetSFI.Machine.
 Require Import TargetSFI.CS.
+Require Import TargetSFI.EitherMonad.
 
 Require Import CompCert.Events.
 
@@ -35,155 +36,6 @@ Import Env.
 Import SFIComponent.
 Import RiscMachine.
 Import CS.
-
-Open Scope string_scope.
-Definition show_pos (p : positive) := show_nat (Pos.to_nat p).
-
-Definition show_value (v : RiscMachine.value) := show_int v.
-
-Definition show_N ( n : N ) := show_nat (N.to_nat n).
-
-Instance show_Component_id : Show Component.id :=
-  {|
-    show := show_pos
-  |}.
-
-Instance show_sfi_id : Show SFIComponent.id :=
-  {|
-    show := show_N
-  |}.
-
-Instance show_CN : Show Env.CN := showList.
-
-Definition show_addr (addr : RiscMachine.address) :=
-  let '(c,s,o) := SFI.convert_address addr in
-  "(c=" ++ (show_N c) ++ ", s=" ++ (show s)
-        ++ ", o=" ++ (show o) ++ ")".
-
-Instance show_addr_i : Show  RiscMachine.address :=
-  {|
-    show := show_addr
-  |}.
-
-Instance show_Addr_Proc : Show (RiscMachine.address * Procedure.id) := showPair.
-
-Instance show_E : Show Env.E := showList.
-
-Instance show_env : Show Env.t :=
-  {
-    show := fun (G : Env.t) =>
-              let (cn,e) := G in 
-              (show cn) ++ (show e)
-  }.
-
-Instance show_event : Show event :=
-  {|
-    show := fun (e : event) =>
-              match e with
-              | ECall c1 pid arg c2 => "[ECall " ++ (show c1) ++ " "
-                                                 ++ (show pid) ++ " "
-                                                 ++ (show_int arg) ++ " "
-                                                 ++ (show c2) ++ "]"
-              |  ERet c1 arg c2 => "[ERet " ++ (show c1) ++ " "
-                                                 ++ (show_int arg) ++ " "
-                                                 ++ (show c2) ++ "]"
-              end
-  |}.
-
-
-
-Definition show_op_f (op : RiscMachine.ISA.binop) :=
-  match op with 
-  | RiscMachine.ISA.Addition => "+"
-  | RiscMachine.ISA.Subtraction => "-"
-  | RiscMachine.ISA.Multiplication => "*"
-  | RiscMachine.ISA.Equality => "="
-  | RiscMachine.ISA.Leq => "<="
-  | RiscMachine.ISA.BitwiseOr => "|"
-  | RiscMachine.ISA.BitwiseAnd => "&"
-  | RiscMachine.ISA.ShiftLeft => "<<"
-  end.
-
-Instance show_op : Show RiscMachine.ISA.binop :=
-  {|
-    show := show_op_f
-  |}.
-
-Instance show_reg : Show RiscMachine.Register.t :=
-  {|
-    show := fun r =>
-              if (N.eqb r RiscMachine.Register.R_ONE)
-              then "R_ONE"
-              else
-                if (N.eqb r Register.R_COM) then "R_COM"
-                else if (N.eqb r Register.R_AUX1) then "R_AUX1"
-                     else if (N.eqb r Register.R_AND_CODE_MASK) then "R_AND_CODE_MASK"
-                          else if (N.eqb r Register.R_AND_DATA_MASK) then "R_AND_DATA_MASK"
-                               else if (N.eqb r Register.R_OR_CODE_MASK) then "R_OR_CODE_MASK"
-                                    else if (N.eqb r Register.R_OR_DATA_MASK) then "R_OR_DATA_MASK"
-                                         else if (N.eqb r Register.R_AUX2) then "R_AUX2"
-                                              else if (N.eqb r Register.R_RA) then "RA"
-                                                   else if (N.eqb r Register.R_SP) then "SP"
-                                                        else if (N.eqb r Register.R_SFI_SP) then "SFI_SP"
-                                                             else if (N.eqb r Register.R_T) then "R_T"
-                                                                  else if (N.eqb r Register.R_D) then "R_D"
-                                                                       else (show_N r)
-  |}.
-
-Instance show_instr : Show RiscMachine.ISA.instr :=
-  {|
-    show := fun i =>
-              match i with
-              | ISA.INop => "Nop"                         
-              (* register operations *)
-              | ISA.IConst v r => ("Const " ++ (show v) ++ " " ++ (show r))%string
-              | ISA.IMov r1 r2  => ("Mov " ++ (show r1) ++ " " ++ (show r2))%string
-              | ISA.IBinOp op r1 r2 r3 => ("BinOP " ++ (show op) ++ " "
-                                                   ++ (show r1) ++ " "
-                                                   ++ (show r2) ++ " "
-                                                   ++ (show r3))%string
-              (* memory operations *)
-              | ISA.ILoad r1 r2 => ("Load " ++ (show r1) ++ " " ++ (show r2))%string
-              | ISA.IStore r1 r2 => ("Store " ++ (show r1) ++ " " ++ (show r2))%string
-              (* conditional and unconditional jumps *)
-              | ISA.IBnz r imm => ("BnZ " ++ (show r) ++ " " ++ (show imm))%string
-              | ISA.IJump r => ("Jump " ++ (show r))%string
-              | ISA.IJal addr=> ("Jal " ++ (show_addr addr))%string
-              (* termination *)
-              | ISA.IHalt => "Halt"
-              end
-  |}.
-
-Definition newline := String "010" ""%string.
-
-
-Instance show_trace : Show trace := showList.
-
-Definition show_mem (mem : RiscMachine.Memory.t) : string :=
-  List.fold_left (fun acc '(a,val) =>
-                    match val with
-                    | RiscMachine.Data v => acc++((show_addr a) ++ ":" ++ (show_value v) ++ newline)%string
-                    | RiscMachine.Instruction i => acc++((show_addr a) ++ ":" ++ (show i) ++ newline)%string
-                    end
-                 ) (BinNatMap.elements mem) ""%string.
-     
-
-Instance show_mem_i : Show RiscMachine.Memory.t :=
-  {|
-    show := show_mem
-  |}.
-
-
-Instance show_state : Show MachineState.t :=
-  {|
-    show := fun (st : MachineState.t) =>
-              let '(mem,pc,gen_regs) := st in
-              "PC: " ++ (show_addr pc) ++ newline
-                     ++ "registers: " ++ (show gen_regs) ++ newline
-                     ++ "memory: " ++ newline ++ (show mem) 
-  |}.
-
-Close Scope string_scope.
 (* TODO Use UPenn MetaLibrary *)
 
 (*******************************
@@ -457,7 +309,7 @@ Definition genRegsAddress (mem : RiscMachine.Memory.t)
            (rptr : RiscMachine.Register.t) (code : bool) : G RiscMachine.RegisterFile.t :=
   let genVal : G RiscMachine.value := arbitrary in
   let rptr_nat := N.to_nat rptr in
-  liftGen3 (fun l1 l2 l3 => l1 ++ l2 ++ l3)
+  liftGen3 (fun l1 l2 l3 => l1 ++ l2 ++ l3)%list
            (vectorOf (rptr_nat - 1) genVal)
            (vectorOf 1 (if code
            then
