TargetSFI/SFIUtil.v
@@ -8,9 +8,24 @@ Require Import Coq.Strings.String.
 Require Import Coq.NArith.BinNat.
 Require Import Coq.PArith.BinPos.
 
+Require Import Coq.FSets.FMapAVL.
+Require Import Coq.FSets.FMapFacts.
+Require Import Coq.Structures.OrdersEx.
+Require Import Coq.Structures.OrdersAlt.
+
 Set Implicit Arguments.
 Set Contextual Implicit.
 
+Module N_as_OT := Backport_OT N_as_OT.
+Module BinNatMap := FMapAVL.Make(N_as_OT).
+Module BinNatMapExtra := WProperties_fun N_as_OT BinNatMap.
+Module BinNatMapFacts := BinNatMapExtra.F.
+
+Module backPositive_as_OT := Backport_OT Positive_as_OT.
+Module PMap := FMapAVL.Make backPositive_as_OT.
+Module PMapExtra := WProperties_fun Positive_as_OT PMap.
+Module PMapFacts := PMapExtra.F.
+  
 Module ListUtil.
 
   Fixpoint get {A:Type} (pos:nat) (l : list A) : option A :=
